theories/program_logic/ectx_lifting.v
@@ -5,7 +5,7 @@ From iris.proofmode Require Import tactics.
 Set Default Proof Using "Type".
 
 Section lifting.
-Context {Λ : ectxLanguage} `{irisDG Λ Σ, invG Σ} {Hinh : Inhabited (state Λ)}.
+Context {Λ : ectxLanguage} `{!irisDG Λ Σ, !invG Σ} {Hinh : Inhabited (state Λ)}.
 Implicit Types v : val Λ.
 Implicit Types e : expr Λ.
 Implicit Types σ : state Λ.
@@ -20,7 +20,7 @@ Lemma dwp_lift_pure_det_head_step {E1 E1' Φ} e1 e1' e2 e2' efs1 efs2 :
   (∀ κ1 σ1 e1'' σ1' efs1', head_step e1 σ1 κ1 e1'' σ1' efs1' → κ1 = [] ∧ σ1' = σ1 ∧ e1'' = e1' ∧ efs1' = efs1) →
   (∀ σ2, head_reducible e2 σ2) →
   (∀ κ2 σ2 e2'' σ2' efs2', head_step e2 σ2 κ2 e2'' σ2' efs2' → κ2 = [] ∧ σ2' = σ2 ∧ e2'' = e2' ∧ efs2' = efs2) →
-  (|={E1,E1'}▷=> dwp E1 e1' e2' Φ ∗
+  (|={E1}[E1']▷=> dwp E1 e1' e2' Φ ∗
                  [∗ list] ef1;ef2 ∈ efs1;efs2, dwp ⊤ ef1 ef2 (λ _ _, True ))
   ⊢ dwp E1 e1 e2 Φ.
 Proof using Hinh.
